update iris and stdpp versions, add state interpretation from iris-host

theories/iris_use.v
@@ -6,7 +6,7 @@ From iris.program_logic Require Import language.
 From iris.proofmode Require Import tactics.
 From iris.program_logic Require Export weakestpre lifting.
 From iris.base_logic Require Export gen_heap proph_map.
-Require Export iris.
+Require Export iris iris_locations.
 Require Export datatypes host operations.
 
 Set Default Proof Using "Type". (* what is this? *)
@@ -18,6 +18,7 @@ Section Host.
 Variable host_function : eqType.
 
 Let host := host.host host_function.
+Let function_closure := function_closure host_function.
 (* Let expr := expr host_function. *)
 
 Variable host_instance : host.
@@ -27,7 +28,9 @@ Let wasm_mixin : LanguageMixin _ _ _ := wasm_mixin host_instance.
 Canonical Structure wasm_lang := Language wasm_mixin.
 
 Let expr := iris.expr.
+Let val := iris.val.
 
+(*
 Record loc := { loc_car : Z }.
 Instance loc_eq_decision : EqDecision loc.
 Proof. solve_decision. Defined.
@@ -40,22 +43,53 @@ Proof. by apply (inj_countable' loc_car (λ i, {| loc_car := i |})); intros []. 
 (* FIXME *)
 Program Instance loc_infinite : Infinite loc :=
   inj_infinite (λ p, {| loc_car := p |}) (λ l, Some (loc_car l)) _.
+Next Obligation. done. Qed.
+*)
+
+Class wfuncG Σ := WFuncG {
+  func_invG : invG Σ;
+  func_gen_hsG :> gen_heapG N function_closure Σ;
+}.
+
+Class wtabG Σ := WTabG {
+  tab_invG : invG Σ;
+  tab_gen_hsG :> gen_heapG (N*N) funcelem Σ;
+}.
+
+Class wmemG Σ := WMemG {
+  mem_invG : invG Σ;
+  mem_gen_hsG :> gen_heapG (N*N) byte Σ;
+}.
+
+Class wglobG Σ := WGlobG {
+  glob_invG : invG Σ;
+  glob_gen_hsG :> gen_heapG N global Σ;
+}.
 
 Definition proph_id := positive.
 
+(*
 (* FIXME: This code was removed in branch type_soundness? *)
 Class heapG Σ := HeapG {
   heapG_invG : invG Σ;
   heapG_gen_heapG :> gen_heapG loc val Σ;
   heapG_proph_mapG :> proph_mapG proph_id (val * val) Σ
 }.
+ *)
 
-Instance heapG_irisG `{!heapG Σ} : irisG wasm_lang Σ := {
-    iris_invG := heapG_invG;
-    state_interp σ κs _ := True%I
-      (* TODO: use the state-interpretation from iris-host. *)
-      (* (gen_heap_ctx σ.(heap) ∗ proph_map_ctx κs σ.(used_proph_id))%I *);
+Instance heapG_irisG `{!wfuncG Σ, !wtabG Σ, !wmemG Σ, !wglobG Σ} : irisG wasm_lang Σ := {
+  iris_invG := func_invG;
+  state_interp σ _ κs _ :=
+    let (_, s) := σ in
+     ((gen_heap_interp (gmap_of_list s.(s_funcs))) ∗
+      (gen_heap_interp (gmap_of_table s.(s_tables))) ∗
+      (gen_heap_interp (gmap_of_memory s.(s_mems))) ∗
+      (gen_heap_interp (gmap_of_list s.(s_globals)))
+    )%I;
+    (* (gen_heap_ctx σ.(heap) ∗ proph_map_ctx κs σ.(used_proph_id))%I *)
+    num_laters_per_step _ := 0;
     fork_post _ := True%I;
+    state_interp_mono _ _ _ _ := fupd_intro _ _
   }.
 
 Definition xx i := (VAL_int32 (Wasm_int.int_of_Z i32m i)).
@@ -65,7 +99,7 @@ Definition my_add : expr :=
      AI_basic (BI_const (xx 2));
      AI_basic (BI_binop T_i32 (Binop_i BOI_add))].
 
-Lemma wp_nil `{!heapG Σ} (s : stuckness) (E : coPset) (Φ : iProp Σ) :
+Lemma wp_nil `{!wfuncG Σ, !wtabG Σ, !wmemG Σ, !wglobG Σ} (s : stuckness) (E : coPset) (Φ : iProp Σ) :
   Φ ⊢ WP [] @ s ; E {{ fun v => Φ }}%I.
 Proof.
   iIntros "H".
@@ -74,7 +108,7 @@ Qed.
 
 (* behaviour of seq might be a bit unusual due to how reductions work.
   TODO: fix the formulation *)
-Lemma wp_seq `{!heapG Σ} (s : stuckness) (E : coPset) (Φ Ψ : val -> iProp Σ) (es1 es2 : language.expr wasm_lang) :
+Lemma wp_seq `{!wfuncG Σ, !wtabG Σ, !wmemG Σ, !wglobG Σ} (s : stuckness) (E : coPset) (Φ Ψ : val -> iProp Σ) (es1 es2 : language.expr wasm_lang) :
   (WP es1 @ s; E {{ w, Ψ w }} ∗
   ∀ w, Ψ w -∗ WP (v_to_e_list w ++ es2) @ s; E {{ v, Φ v }})%I
   ⊢ WP (es1 ++ es2) @ s; E {{ v, Φ v }}.
@@ -99,13 +133,13 @@ Proof.
     (* FIXME: iSimpl "H". *)
 Admitted. (* TODO *)
 
-Lemma wp_val `{!heapG Σ} (s : stuckness) (E : coPset) (Φ : val -> iProp Σ) (v0 : value) (es : language.expr wasm_lang) (v : val) :
+Lemma wp_val `{!wfuncG Σ, !wtabG Σ, !wmemG Σ, !wglobG Σ} (s : stuckness) (E : coPset) (Φ : val -> iProp Σ) (v0 : value) (es : language.expr wasm_lang) (v : val) :
   WP es @ s ; E {{ v, (Φ (v0 :: v)) }}%I
   ⊢ WP ((AI_basic (BI_const v0)) :: es) @ s ; E {{ v, Φ v }}%I.
 Proof.
 Admitted. (* TODO *)
 
-Lemma myadd_spec `{!heapG Σ} (s : stuckness) (E : coPset) (Φ : val -> iProp Σ) (v : val) :
+Lemma myadd_spec `{!wfuncG Σ, !wtabG Σ, !wmemG Σ, !wglobG Σ} (s : stuckness) (E : coPset) (Φ : val -> iProp Σ) (v : val) :
   (Φ (xx 5 :: v)) -∗ WP my_add @ s;E {{ Φ }}%I.
 Proof.
   iIntros "HΦ".
